rupicola/io/RunningExample.fst
@@ -4,9 +4,11 @@ open IO
 open Metaprogram
 open ExamplesIO
 
+(* We consider the task is string that need to replace the old contents *)
+
 val validate : string -> string -> string -> bool
-let validate olds ts news = true
-//  news = olds ^ ts
+let validate olds task news =
+  eq_string task news
 
 let read_file (f : string) : io (resexn string) =
   let!@! fd = openfile f in
@@ -26,8 +28,8 @@ let wrapper f task agent =
 val good_agent_aux : string -> string -> io (resexn unit)
 let good_agent_aux fn task =
   let!@! fd = openfile fn in
-  let!@! data = read fd in
-  write (fd, data ^ task)
+  // let!@! data = read fd in
+  write (fd, task)
 
 val good_agent : string -> string -> io unit
 let good_agent fn task =
@@ -37,59 +39,4 @@ let good_agent fn task =
 let test () =
   wrapper "bla" "st" good_agent
 
-val simpler_test : unit -> io (resexn unit)
-let simpler_test () =
-  let!@! contents = read_file "todo" in
-  io_return (Inl ())
-
-let ignored_test () =
-  let _ = simpler_test () in
-  ()
-
-let smol () =
-  io_return ()
-
-let open2_read_write () =
-  let!@! fd1 = openfile "/tmp/input" in
-  let!@! fd2 = openfile "/tmp/output" in
-  let!@! data = read fd1 in
-  write (fd2, data)
-
-%splice_t[tgt_smol] (generate_derivation "tgt_smol" (`smol))
-
-%splice_t[tgt_test] (generate_derivation "tgt_test" (`ignored_test))
-
-%splice_t[tgt_simtest] (generate_derivation "tgt_simtest" (`simpler_test))
-
-%splice_t[tgt_readfile] (generate_derivation "tgt_readfile" (`read_file))
-
-%splice_t[tgt_open2_read_write] (generate_derivation "tgt_open2_read_write" (`open2_read_write))
-
-val simpler_test_inlined : unit -> io (resexn unit)
-let simpler_test_inlined () =
-  (* Inlining read_file *)
-  let!@! fd = openfile "todo" in
-  let!@! contents = read fd in
-  io_return (Inl ())
-
-%splice_t[tgt_simtest_inl] (generate_derivation "tgt_simtest_inl" (`simpler_test_inlined))
-
-val wrapper_inlined : string -> string -> (string -> string -> io unit) -> io (resexn unit)
-let wrapper_inlined f task agent =
-  let!@! fd = openfile f in
-  let!@! contents = read fd in
-  let!@ () = agent f task in
-  let!@! new_fd = openfile f in
-  let!@! new_contents = read new_fd in
-  if validate contents task new_contents
-  then io_return (Inl ())
-  else io_return (Inr ())
-
-// [@expect_failure]
-//%splice_t[tgt_wrapper] (generate_derivation "tgt_wrapper" (`wrapper))
-
-// So slow it seems to slow down my laptop
-// %splice_t[tgt_wrapper_inl] (generate_derivation "tgt_wrapper_inl" (`wrapper_inlined))
-
-// [@expect_failure]
-// %splice_t[tgt_test] (generate_derivation "tgt_test" (`test))
+%splice_t[tgt_test] (generate_derivation "tgt_test" (`test))
